io/ILang.fst
@@ -23,11 +23,11 @@ open TC.Monitorable.Hist
 
 
   
-unfold let pi_hist (a:Type) (pi:monitorable_prop) : Hist.hist a =
+unfold let pi_hist (#a:Type) (pi:monitorable_prop) : Hist.hist a =
   (fun p h -> forall r lt. enforced_locally pi h lt ==> p lt r)
 
 effect IIOpi (a:Type) (pi : monitorable_prop) = 
-  IIO.IIOwp a (pi_hist a pi)
+  IIO.IIOwp a (pi_hist #a pi)
 
 class ilang (t:Type u#a) (pi:monitorable_prop) = { mldummy : unit }
 
